Progress in sketching compiler_simulation_proof for thread steps.

concurrency/compiler/concurrent_compiler_simulation_proof.v
@@ -24,13 +24,14 @@ Require Import VST.concurrency.common.x86_context.
 
 (** *One thread simulation*)
 Module ThreadedSimulation (CC_correct: CompCert_correctness).
-  
+   
   Import HybridMachineSig.
   Import DryHybridMachine.
 
   Existing Instance OrdinalPool.OrdinalThreadPool.
   Existing Instance HybridMachineSig.HybridCoarseMachine.DilMem.
 
+  Section ThreadedSimulation.
   (** *C Semantics*)
   Context (C_program: Clight.program).
   Definition Clight_g : Clight.genv := Clight.globalenv C_program.
@@ -289,7 +290,26 @@ Module ThreadedSimulation (CC_correct: CompCert_correctness).
           ocd = Some cd ->
           match_thread_compiled cd j s1 m1 s2 m2 ->
           individual_match ocd i j s1 m1 s2 m2.
+
+    Lemma simulation_equivlanence:
+      forall s3 t s2 cd cd0,
+        (Smallstep.plus (Asm.step (Genv.globalenv Asm_program)) 
+                        s3 t s2 \/
+         Smallstep.star (Asm.step (Genv.globalenv Asm_program)) 
+                        s3 t s2 /\ Injorder compiler_sim cd cd0) ->
+        Smallstep.plus (Asm.step (Genv.globalenv Asm_program)) 
+                       s3 t s2 \/
+        t = Events.E0 /\
+        s2 = s3 /\
+        Injorder compiler_sim cd cd0.
+    Proof.
+      intros. destruct H; eauto.
+      destruct H.
+      inversion H; subst; eauto.
+      left. econstructor; eauto.
+    Qed.
     
+    (* This lemma is only used when updating non compiled threads *)
     Lemma Concur_update:
       forall (st1 : t) (m1 m' : mem) (tid : nat) (Htid : containsThread st1 tid)
         c1 (cd cd' : option compiler_index) (st2 : t) 
@@ -305,25 +325,122 @@ Module ThreadedSimulation (CC_correct: CompCert_correctness).
                      (updThread Htid' c2
                                 (getCurPerm m2', snd (getThreadR Htid'))) m2'.
     Proof.
+      
+      (*There is probably a relation missing from m1 m' m2 m2' *)
+      (* Probably it's mem_step* which is provable from where this lemma is used. *)
+    Admitted.
+
+    (*This lemma is used when the compiled thread steps*)
+    Lemma Concur_update_compiled:
+              forall (st1 : t) (m1 m' : mem) (Htid : containsThread st1 hb) 
+                     (st2 : t) (mu : meminj) (m2 : mem) (cd0 : compiler_index),
+                concur_match (Some cd0) mu st1 m1 st2 m2 ->
+                forall (s' : Clight.state) (j1' : meminj) (cd' : Injindex compiler_sim)
+                       (j2' : meminj) (s4' : Asm.state) (j3' : meminj) (m4' : mem)
+                       (Htid' : containsThread st2 hb),
+                  match_thread_compiled cd' (compose_meminj (compose_meminj j1' j2') j3')
+                                        (Krun (SState Clight.state Asm.state s')) m'
+                                        (Krun (TState Clight.state Asm.state s4')) m4' ->
+                  concur_match (Some cd') (compose_meminj (compose_meminj j1' j2') j3')
+                               (updThread Htid (Krun (SState Clight.state Asm.state s'))
+                                          (getCurPerm m', snd (getThreadR Htid))) m'
+                               (updThread Htid' (Krun (TState Clight.state Asm.state s4'))
+                                          (getCurPerm m4', snd (getThreadR Htid'))) m4'.
+            Proof.
+      (*There is probably a relation missing from m1 m' m2 m2' *)
+              (* Probably it's mem_step* which is provable from where this lemma is used. *)
+            Admitted.
+            
+
+    
+    Ltac exploit_match:=
+      unfold match_thread_target,match_thread_source,match_thread_compiled in *;
+      match goal with
+      | [ H: getThreadC ?i = _ ?c,
+             H0: context[match_state2match_thread] |- _ ] =>
+        rewrite H in H0; inversion H0; subst; simpl in *; clear H0
+      end;
+      fold match_thread_target in *;
+      fold match_thread_source in *;
+      fold match_thread_compiled in *.
+
+    (* Build the concur_match *)
+    Ltac destroy_ev_step_sum:=
+      match goal with
+      | [ H: ev_step_sum _ _ _ _ _ _ _ |- _ ] => inversion H; clear H
+      end.
+
+    
+    Inductive corestep_star
+              {state : Type}
+              (step : state -> mem -> state -> mem -> Prop)
+      : state -> mem -> state -> mem -> Prop :=
+      star_refl : forall s m, corestep_star step s m s m
+    | star_step : forall (s1 : state) m1 (s2 : state) m2
+                    (s3 : state) m3,
+        step s1 m1 s2 m2 ->
+        corestep_star step s2 m2 s3 m3 ->
+        corestep_star step s1 m1 s3 m3.
+    Inductive corestep_plus
+              (state : Type) (step : state -> mem -> state -> mem -> Prop)
+      : state -> mem -> state -> mem -> Prop :=
+    | plus_left : forall (s1 : state) m1 (s2 : state) 
+                    m2 (s3 : state) m3,
+        step s1 m1 s2 m2 ->
+        corestep_star step s2 m2 s3 m3 ->
+        corestep_plus state step s1 m1 s3 m3.
+
+    Lemma self_simulation_plus:
+      forall state coresem
+        (SIM: self_simulation.self_simulation state coresem),
+      forall (f : meminj) (t : Events.trace) (c1 : state) 
+        (m1 : mem) (c2 : state) (m2 : mem),
+        self_simulation.match_self (self_simulation.code_inject _ _ SIM) f c1 m1 c2 m2 ->
+        forall (c1' : state) (m1' : mem),
+          (corestep_plus _ (core_semantics.corestep coresem)) c1 m1 c1' m1' ->
+          exists (c2' : state) (f' : meminj) (t' : Events.trace) 
+            (m2' : mem),
+                (corestep_plus _ (core_semantics.corestep coresem)) c2 m2 c2' m2' /\
+                self_simulation.match_self (self_simulation.code_inject _ _ SIM) f' c1' m1' c2' m2' /\
+                self_simulation.is_ext f (Mem.nextblock m1) f' (Mem.nextblock m2) /\
+                Events.inject_trace f' t t'.
     Admitted.
 
     
-        Ltac exploit_match:=
-        unfold match_thread_target,match_thread_source,match_thread_compiled in *;
-        match goal with
-        | [ H: getThreadC ?i = _ ?c,
-               H0: context[match_state2match_thread] |- _ ] =>
-          rewrite H in H0; inversion H0; subst; simpl in *
-        end;
-        fold match_thread_target in *;
-        fold match_thread_source in *;
-        fold match_thread_compiled in *.
+            Lemma thread_step_plus_from_corestep:
+              forall (m : option mem) (tge : ClightSemantincsForMachines.G * Asm.genv)
+                     (U : list nat) (st1 : t) (m1 : mem) (Htid : containsThread st1 hb) 
+                     (st2 : t) (mu : meminj) (m2 : mem) (cd0 : compiler_index)
+                     (H0 : concur_match (Some cd0) mu st1 m1 st2 m2) (code2 : Asm.state)
+                     (s4' : Smallstep.state (Asm.part_semantics Asm_g)) 
+                     (m4' : mem),
+                corestep_plus (Smallstep.state (Asm.part_semantics Asm_g))
+                              (core_semantics.corestep (Asm_core.Asm_core_sem Asm_g)) code2
+                              (restrPermMap
+                                 (proj1 ((memcompat2 (Some cd0) mu st1 m1 st2 m2 H0) hb (contains12 H0 Htid))))
+                              s4' m4' ->
+                forall Htid' : containsThread st2 hb,
+                  machine_semantics_lemmas.thread_step_plus (HybConcSem (Some (S hb)) m) tge U st2
+                                                            m2
+                                                            (updThread Htid' (Krun (TState Clight.state Asm.state s4'))
+                                                                       (getCurPerm m4', snd (getThreadR Htid'))) m4'.
+            Proof.
+              (** NOTE: This might be missing that the corestep never reaches an at_external
+                  If this is the case, we might need to thread that through the compiler...
+                  although it should be easy, I would prefere if there is any other way...
+              *)
+            Admitted.
 
-        (* Build the concur_match *)
-        Ltac destroy_ev_step_sum:=
-          match goal with
-          | [ H: ev_step_sum _ _ _ _ _ _ _ |- _ ] => inversion H; subst
-          end.
+        (** *Need an extra fact about simulations*)
+          Lemma step2corestep_plus:
+            forall (s1 s2: Smallstep.state (Asm.part_semantics Asm_g)) m1 t,
+            Smallstep.plus
+                (Asm.step (Genv.globalenv Asm_program))
+                (Smallstep.set_mem s1 m1) t s2 ->
+            (corestep_plus _ (core_semantics.corestep (Asm_core.Asm_core_sem Asm_g)))
+              s1 m1 s2 (Smallstep.get_mem s2).
+          Admitted.
+        
         
     (* When a thread takes an internal step (i.e. not changing the schedule) *)
     Lemma internal_step_diagram:
@@ -353,7 +470,7 @@ Module ThreadedSimulation (CC_correct: CompCert_correctness).
         pose proof (mtch_target _ _ _ _ _ _ H0 _ l Htid (contains12 H0 Htid)) as HH.
         simpl in *.
         exploit_match.
-        destroy_ev_step_sum; simpl in *.
+        destroy_ev_step_sum; subst; simpl in *.
         simpl.
         eapply Asm_event.asm_ev_ax1 in H2.
         replace Hcmpt with (memcompat1 cd mu st1 m1 st2 m2 H0) in H2 by eapply Axioms.proof_irr.
@@ -399,17 +516,103 @@ Module ThreadedSimulation (CC_correct: CompCert_correctness).
         pose proof (mtch_compiled _ _ _ _ _ _ H0 _ e Htid (contains12 H0 Htid)) as HH.
         destruct HH as (cd0 & H1 & ?).
         subst.
-
-        (* This takes three styeps*)
+        simpl in *; exploit_match. 
         
-        admit. (*Compiler case*)
+        (* This takes three steps:
+           - Simulation of the Clight semantics  
+           - Simulation of the compiler (Clight and Asm) 
+           - Simulation of the Asm semantics 
+         *)
 
+        inversion H6. subst cd j s1 s4.
+        rename H1 into CMatch.
+        rename H3 into Compiler_Match.
+        rename H5 into AsmMatch.
+        simpl in *.
+
+        
+        (* (1) Clight step *)
+        destroy_ev_step_sum. subst m'0 t0 s.
+        eapply (event_semantics.ev_step_ax1 (@semSem CSem)) in H3; eauto.
+        replace Hcmpt with (memcompat1 (Some cd0) mu st1 m1 st2 m2 H0) in H3
+          by eapply Axioms.proof_irr.
+        
+        eapply Cself_simulation in H3; eauto.
+        destruct H3 as (c2' & j1' & t' & m2' & (CoreStep & MATCH & is_ext & inject_incr)).
+        
+        (* (2) Compiler step/s *)
+        inversion CoreStep. subst s1 m7 s0 m8.
+        eapply compiler_sim in H1; simpl in *; eauto.
+        destruct H1 as (cd' & s2' & j2' & t'' & step & comp_match & INJ_incr & inj_event).
+
+        eapply simulation_equivlanence in step.
+        destruct step as [plus_step | (? & ? & ?)].
+        
+        + (*Case: assembly takes at least one step *)
+          eapply step2corestep_plus in plus_step.
+
+          (* (3) Asm simulation (extended to multiple steps)  *)
+          eapply (self_simulation_plus _ _ Aself_simulation) in plus_step; eauto.
+          destruct plus_step as (s4' & j3' & t3 & m4' & CstepPlus & AMatch & ? & inj_trace).  
+          
+          (* contains.*)
+          pose proof (@contains12  _ _ _ _ _ _  H0 _ Htid) as Htid'.
+          (* Construct the new thread pool *)
+          exists (updThread Htid' (Krun (TState Clight.state Asm.state s4'))
+                       (getCurPerm m4', snd (getThreadR Htid'))).
+          (* new memory is given by the self_simulation. *)
+          exists m4', (Some cd'), (compose_meminj (compose_meminj j1' j2') j3').
+          split; [|left].
+          * (* Reconstruct the match *)
+          
+            simpl in *.
+            eapply Concur_update_compiled; eauto.
+
+            (* match_thread_compiled *)
+            {
+unfold match_thread_compiled.
+              econstructor.
+              econstructor; eauto.
+              move comp_match at bottom.
+              simpl in comp_match.
+              unfold compiler_match.
+              match goal with
+              | [  |- context[Injmatch_states _ _ _ _ ?X] ] =>
+                replace X with s2' by (destruct s2'; reflexivity)
+              end. 
+              eauto.
+            }
+          * eapply thread_step_plus_from_corestep; eauto.
+            
+        + (*Reestablish the concur_match *)
+          simpl.
+          move H0 at bottom.
+          eapply Concur_update; eauto.
+          econstructor 1; eauto.
+          simpl in MATCH.
+          unfold match_thread_source; simpl.
+          constructor.
+          exact MATCH.
+        + (* Construct the step *)
+          exists 0; simpl.
+          do 2 eexists; split; [|reflexivity].
+          replace m2' with (HybridMachineSig.diluteMem m2') by reflexivity.
+          econstructor; eauto; simpl.
+          econstructor; eauto.
+          * simpl in *.
+            eapply H0.
+          * simpl. econstructor; eauto.
+          * simpl; repeat (f_equal; try eapply Axioms.proof_irr).
+        
+        
+        
+        admit. 
         
       - (* tid > hb *)
         pose proof (mtch_source _ _ _ _ _ _ H0 _ l Htid (contains12 H0 Htid)) as HH.
         simpl in *.
         exploit_match.
-        destroy_ev_step_sum; simpl in *.
+        destroy_ev_step_sum; subst; simpl in *.
         simpl.
         eapply (event_semantics.ev_step_ax1 (@semSem CSem)) in H2; eauto.
         replace Hcmpt with (memcompat1 cd mu st1 m1 st2 m2 H0) in H2
@@ -588,7 +791,8 @@ Module ThreadedSimulation (CC_correct: CompCert_correctness).
     apply CC_correct.simpl_clight_semantic_preservation in H.
     unfold ClightMachine.ClightMachine.DMS.ClightConcurSem, HybridMachineSig.HybridMachineSig.ConcurMachineSemantics, ClightMachine.ClightMachine.DMS.ClightMachine, HybridMachineSig.HybridMachineSig.HybridCoarseMachine.HybridCoarseMachine.
     econstructor.
-*)
+ *)
+ End ThreadedSimulation.
 End ThreadedSimulation.
  
 
